# Parseval identity
Created:2024-02-07 22-39

What we want to understand now is really about momentum space. So we can ask the following question. What happens to the normalization condition that we have for the wave function, when we think in momentum variables?
$\int \Psi^{*} \Psi d x=1$ what about $\int d k \Phi^{*} \Phi=$
$$\int d x \underbrace{\Psi(x)^{*}}_{k} \underbrace{\Psi(x)}_{k^{\prime}}=\int d x \underbrace{\frac{1}{\sqrt{2 \pi}} \int d k \;\Phi^{*}(k) e^{-i k x} \frac{1}{\sqrt{2} \pi} \int d k^{\prime} \Phi\left(k^{\prime}\right) e^{i k^{\prime} x}}_{\psi^{*}}$$
$k$ and $k'$  integral's have no chance because they are abstract integrals. Maybe $d x$ integral does have a chance

$$
\begin{aligned}
& =\int d k \Phi^{*}(k) \int d k^{\prime} \Phi\left(k^{\prime}\right) \underbrace{\frac{1}{2 \pi} \int d x e^{i\left(k^{\prime}-k\right) x}}_{\delta\left(k^{\prime}-k\right)} \\
& =\int d k \Phi^{*}(k) \int d k^{\prime} \Phi\left(k^{\prime}\right) \delta\left(k^{\prime}-k\right) \\
& =\int d k \Phi^{*}(k) \Phi(k)
\end{aligned}
$$

## Parseval theorem (plancherel theorem)

$$
\int d x|\Psi(x)|^{2}=\int d k|\Phi(k)|^{2}
$$

$\Phi(k)$ not only represents the weight with which you superimpose plane wave, but now it also satisfies a normalization condition. $\Phi(k)$ could be thought maybe as a probability distribution, in this new space, in momentum space.

I want to make momentum space a little bit more clear. And this involves a little bit of moving around with constants, but it's important.
We've been using $k$ all the time and $p=\hbar k$. But now let's put things in terms of momentum. Let's do every thing with momentum itself.

## Go to the momentum language:

$$
\begin{aligned}
& p=\hbar k \rightarrow \frac{d p}{\hbar}=d k \\
& \Phi(k)=\tilde{\Phi}(p) \\
& \Psi(x)=\frac{1}{\sqrt{2 \pi}} \int \tilde{\Phi}(p) e^{i p x / \hbar} \frac{d p}{\hbar} \\
& \tilde{\Phi}(p)=\frac{1}{\sqrt{2 \pi}} \int \Psi(x) e^{-i p x / \hbar} d x
\end{aligned}
$$

- wictr√©s fie ty la virus
![](https://cdn.mathpix.com/cropped/2025_05_27_372755343f148c881602g-5.jpg?height=69&width=296&top_left_y=1088&top_left_x=1424)

This thing are not completely symmetric, so were going to do one more little change for more symmetry. Redefine

$$
\tilde{\Phi}(p) \rightarrow \underbrace{\Phi(p)}_{\text{that should n't be confused with the $\Phi(k)$}} \sqrt{h}
$$


put it in the above:

$$
\begin{aligned}
& \Psi(x)=\frac{1}{\sqrt{2 \pi \hbar}} \int \Phi(p) e^{i p x / \hbar} d p \\
& \tilde{\Phi}(p)=\Phi(p) \sqrt{\hbar}=1 / \int_{\sqrt{2 \pi}} \Psi(x) e^{-i p x} \hbar d x \\
& \Phi(p)=\frac{1}{\sqrt{2 \pi \hbar}} \int \Psi(x) e^{-i p x / \hbar} d x \\
& \text { Fourier's theorem in momentum notation } \\
& \Rightarrow \quad \Psi(x)=\frac{1}{\sqrt{2 \pi \hbar}} \int \Phi(p) e^{\frac{i p x}{\hbar}} d p \\
& \Phi(p)=\frac{1}{\sqrt{2 \pi \hbar}} \int \Psi(x) e^{-i p x} / \hbar d x
\end{aligned}
$$

## References:36

## Related:



